Change FStar.SnapshotHyperStack to use FStar.Monotonic.HyperStack

ulib/FStar.SnapshotHyperStack.fst
@@ -1,12 +1,14 @@
 module FStar.SnapshotHyperStack
 
+open FStar.Preorder
+open FStar.DataInvariant
 open FStar.HyperHeap
-open FStar.HyperStack
+open FStar.Monotonic.HyperStack
 
-module HS = FStar.HyperStack
+module HS = FStar.Monotonic.HyperStack
 module HH = FStar.HyperHeap
 
-type snapshot_heap = (HS.mem * option HS.mem)
+abstract type snapshot_heap = (HS.mem * option HS.mem)
 
 let is_unrestricted (h : snapshot_heap) : bool =
 Some? (snd h)
@@ -38,7 +40,10 @@ let lemma_equal_stack_domains_trans (m0 m1 m2 : snapshot_heap) : Lemma
 let heap (m:snapshot_heap) : hh =
 (active_mem m).HS.h
 
-let tip (m:snapshot_heap) : tip:rid {tip `HS.is_tip` (active_mem m).h} =
+let is_tip (id : rid) (mem : snapshot_heap) : Type0 =
+HS.is_tip id (heap mem)
+
+let tip (m:snapshot_heap) : tip:rid {tip `is_tip` m} =
 (active_mem m).HS.tip
 
 // let am = active_mem m in am.tip
@@ -59,25 +64,33 @@ match h with
 let popped (h0 h1 : snapshot_heap) =
 HS.popped (active_mem h0) (active_mem h1)
 
-let upd (#a:Type) (m: snapshot_heap) (s:HS.reference a {HS.live_region (active_mem m) s.HS.id}) (v:a) : GTot snapshot_heap =
+let live_region (mem : snapshot_heap) (id : rid) : Type0 =
+HS.live_region (active_mem mem) id
+
+let sel (#a:Type) (#rel:preorder a) (m: snapshot_heap) (s:HS.mreference a rel) : GTot a =
+(active_mem m).h.[s.ref]
+
+let upd
+  (#a:Type)
+  (#rel:preorder a)
+  (m: snapshot_heap)
+  (s:HS.mreference a rel {live_region m s.HS.id})
+  (v:a { rel (sel m s) v }) : GTot snapshot_heap =
 match m with
 | (h0, None) -> (HS.upd h0 s v, None)
 | (h0, Some h1) -> (h0, Some (HS.upd h1 s v))
 
-let sel (#a:Type) (m: snapshot_heap) (s:reference a) : GTot a =
-(active_mem m).h.[s.ref]
-
-let contains (#a:Type) (m: snapshot_heap) (s: HS.reference a) =
+let contains (#a:Type) (#rel:preorder a) (m: snapshot_heap) (s: HS.mreference a rel) =
 HS.contains (active_mem m) s
 
-let unused_in (#a:Type) (r:reference a) (h:snapshot_heap) =
+let unused_in (#a:Type) (#rel:preorder a) (r:HS.mreference a rel) (h:snapshot_heap) =
   HS.unused_in r (active_mem h)
 
 let modifies_one id h0 h1 = HS.modifies_one id (active_mem h0) (active_mem h1)
 let modifies_ref (id:rid) (s:Set.set nat) (h0 h1 : snapshot_heap) =
   HS.modifies_ref id s (active_mem h0) (active_mem h1)
 
-let lemma_upd_1 #a (h:snapshot_heap) (x:reference a) (v:a) : Lemma
+let lemma_upd_1 #a (#rel:preorder a) (h:snapshot_heap) (x:HS.mreference a rel) (v:a{ rel (sel h x) v }) : Lemma
    (requires (contains h x))
    (ensures (contains h x
              /\ modifies_one (frameOf x) h (upd h x v)
@@ -86,7 +99,7 @@ let lemma_upd_1 #a (h:snapshot_heap) (x:reference a) (v:a) : Lemma
     [SMTPat (upd h x v); SMTPatT (contains h x)]
     = ()
 
-let lemma_upd_2 (#a:Type) (h:snapshot_heap) (x:reference a) (v:a) : Lemma
+let lemma_upd_2 (#a:Type) (#rel:preorder a) (h:snapshot_heap) (x:HS.mreference a rel) (v:a{rel (sel h x) v}) : Lemma
    (requires (frameOf x = (tip h) /\ x `unused_in` h))
    (ensures (frameOf x = (tip h)
             /\ modifies_one (tip h) h (upd h x v)
@@ -95,23 +108,23 @@ let lemma_upd_2 (#a:Type) (h:snapshot_heap) (x:reference a) (v:a) : Lemma
     [SMTPat (upd h x v); SMTPatT (x `unused_in` h)]
     = ()
 
-val lemma_live_1: #a:Type ->  #a':Type -> h:snapshot_heap -> x:reference a -> x':reference a' -> Lemma
+val lemma_live_1: #a:Type -> #a':Type -> #rel1:preorder a -> #rel2:preorder a' -> h:snapshot_heap -> x:HS.mreference a rel1 -> x':mreference a' rel2 -> Lemma
 (requires (contains h x /\ x' `unused_in` h))
 (ensures  (x.id <> x'.id \/ ~ (as_ref x === as_ref x')))
 [SMTPat (contains h x); SMTPat (x' `unused_in` h)]
-let lemma_live_1 #a #a' h x x' = ()
+let lemma_live_1 #a #a' #rel1 #rel2 h x x' = ()
 
-unfold let hs_remove_reference (#a:Type) (r:reference a) (m:mem{m `HS.contains` r /\ is_mm r}) :GTot mem =
+unfold let hs_remove_reference (#a:Type) (#rel:preorder a) (r:HS.mreference a rel) (m:mem{m `HS.contains` r /\ is_mm r}) :GTot mem =
   let h_0 = Map.sel m.h r.id in
   let h_1 = Heap.free_mm h_0 (HH.as_ref r.ref) in
   HS (Map.upd m.h r.id h_1) m.tip
 
-let remove_reference (#a:Type) (r:HS.reference a) (m:snapshot_heap {m `contains` r /\ is_mm r}) : GTot snapshot_heap =
+let remove_reference (#a:Type) (#rel:preorder a) (r:HS.mreference a rel) (m:snapshot_heap {m `contains` r /\ is_mm r}) : GTot snapshot_heap =
 match m with
 | (h0, None) -> (hs_remove_reference r h0, None)
 | (h0, Some h1) -> (h0, Some (hs_remove_reference r h1))
 
-let weak_contains (#a:Type) (m: snapshot_heap) (s: HS.reference a) =
+let weak_contains (#a:Type) (#rel:preorder a) (m: snapshot_heap) (s: HS.mreference a rel) =
   HS.weak_contains (active_mem m) s
 
 let modifies (s : Set.set rid) (m0 m1 : snapshot_heap) =
